Make sures it compiles with Dafny 4.6.

helper.dfy
@@ -4,30 +4,30 @@ newtype {:nativeType "byte"} byte = x : int | 0 <= x < 256
 newtype {:nativeType "uint"} uint32 = x : int | 0 <= x < 4294967296
 
 // modular arithmetic
-function method add_byte(x : byte, y : byte) : byte
+function add_byte(x : byte, y : byte) : byte
 {
   ((x as int + y as int) % 256) as byte
 }
 
 // modular arithmetic
-function method sub_byte(x : byte, y : byte) : byte
+function sub_byte(x : byte, y : byte) : byte
 {
   (((x as int) + (256 - y as int)) % 256) as byte
 }
 
 lemma add_sub(x : byte, y : byte)
-  ensures sub_byte(add_byte(x, y), y) == x;
+  ensures sub_byte(add_byte(x, y), y) == x
 {
 }
 
-function method byte_from(x : int) : byte
+function byte_from(x : int) : byte
 {
   (x % 256) as byte
 }
 
 // uint32 as sequence of 4 bytes
-function method unpack(x : uint32) : seq<byte>
-  ensures |unpack(x)| == 4;
+function unpack(x : uint32) : seq<byte>
+  ensures |unpack(x)| == 4
 {
   var b0 : byte := ((x / (256 * 256 * 256)) % 256) as byte;
   var b1 : byte := ((x / (256 * 256)) % 256) as byte;
@@ -37,19 +37,19 @@ function method unpack(x : uint32) : seq<byte>
 }
 
 // 4 bytes as uint32
-function method pack(x : seq<byte>) : uint32
-  requires |x| == 4;
+function pack(x : seq<byte>) : uint32
+  requires |x| == 4
 {
   (x[0] as uint32) * 16777216 + (x[1] as uint32) * 65536 + (x[2] as uint32) * 256 + (x[3] as uint32)
 }
 
 lemma pack_unpack(x : seq<byte>)
-  requires |x| == 4;
-  ensures unpack(pack(x)) == x;
+  requires |x| == 4
+  ensures unpack(pack(x)) == x
 {
 }
 
 lemma unpack_pack(x : uint32)
-  ensures pack(unpack(x)) == x;
+  ensures pack(unpack(x)) == x
 {
 }
